test/CircuitTest.lean
@@ -1,0 +1,56 @@
+import Runwai.Typing
+
+@[simp]
+def assertCircuit : Ast.Circuit := {
+  name   := "assert",
+  inputs := ("trace", Ast.Ty.refin (Ast.Ty.arr (Ast.Ty.refin (Ast.Ty.arr (Ast.Ty.refin Ast.Ty.field (Ast.Predicate.const (Ast.Expr.constBool true))) 2) (Ast.Predicate.const (Ast.Expr.constBool True))) 2) (Ast.Predicate.const (Ast.Expr.constBool true))),
+  output := ("u", Ast.Ty.refin (Ast.Ty.unit)
+                      (Ast.Predicate.const (Ast.Expr.binRel
+                        (Ast.Expr.arrIdx (Ast.Expr.arrIdx (Ast.Expr.var "trace") (Ast.Expr.constF 1)) (Ast.Expr.constF 0))
+                        Ast.RelOp.eq
+                        (Ast.Expr.constF 2)))),
+  body   := (Ast.Expr.letIn "u" (Ast.Expr.assertE
+              (Ast.Expr.arrIdx (Ast.Expr.arrIdx (Ast.Expr.var "trace") (Ast.Expr.constF 1)) (Ast.Expr.constF 0))
+              (Ast.Expr.constF 2))
+            (Ast.Expr.var "u"))
+}
+
+def Δ : Env.CircuitEnv := [("assert", assertCircuit)]
+
+theorem assertCircuit_correct : (Ty.circuitCorrect Δ assertCircuit) := by
+  unfold Ty.circuitCorrect
+  unfold assertCircuit
+  simp_all
+  intro x hs hi hσ
+  set envs := Ty.makeEnvs assertCircuit x
+  set σ := envs.1
+  set Γ := envs.2
+  apply Ty.TypeJudgment.TE_LetIn
+  apply Ty.TypeJudgment.TE_Assert
+  apply Ty.TypeJudgment.TE_ArrayIndex
+  apply Ty.TypeJudgment.TE_ArrayIndex
+  apply Ty.TypeJudgment.TE_Var
+  unfold Ty.makeEnvs
+  unfold Env.updateTy
+  unfold Env.lookupTy
+  simp_all
+  constructor
+  . constructor
+    . constructor
+      . constructor
+        . rfl
+        . rfl
+      . rfl
+    . rfl
+  . rfl
+  apply Eval.EvalProp.ConstF
+  simp_all
+  apply Eval.EvalProp.ConstF
+  simp_all
+  apply Ty.TypeJudgment.TE_ConstF
+  apply Ty.TypeJudgment.TE_VarEnv
+  unfold Env.updateTy
+  unfold Env.lookupTy
+  simp_all
+  unfold Ast.exprEq
+  rfl
